src/isabelle/tr/Insert.thy
@@ -1,0 +1,71 @@
+theory Insert
+imports Common
+begin
+
+section types
+
+datatype ('r) stk = Stk "('r page_ref * nat) list"
+
+section "parameters"
+
+section "insert,  ins_state, ins_step"
+
+record ('bs,'k,'r,'v) ins_state_down = 
+  isd_k :: "'k key"
+  isd_v :: "'v value_t"
+  isd_r :: "'r page_ref"
+  isd_stk :: "'r stk"
+  isd_str :: "('r,'bs) store"
+
+record ('r) ins_state_up_1 = 
+  isu1_r :: "'r page_ref"
+  
+(* r1 <= k < r2 *)
+record ('k,'r,'v) ins_state_up_2 = 
+  isu2_r1 :: "'r page_ref"
+  isu2_k :: "'k key"
+  isu2_r2 :: "'r page_ref"
+
+datatype ('k,'r,'v) ins_state_up' = 
+  S "'r ins_state_up_1"  (* inserting a single pointer *)
+  | D "('k,'r,'v) ins_state_up_2"  (* inserting two pointers, separated by a key *)
+
+record ('bs,'k,'r,'v) ins_state_up =
+  isu_s :: "('k,'r,'v) ins_state_up'"
+  isu_stk :: "'r stk"
+  isu_str :: "('bs,'r) store"
+
+datatype ('bs,'k,'r,'v) ins_state = 
+  Down "('bs,'k,'r,'v) ins_state_down"
+  | Up "('bs,'k,'r,'v) ins_state_up"
+
+
+definition ins_step :: "('bs,'k,'r,'v) ctxt_k2r_t
+  => ('bs,'k,'r,'v) ins_state 
+  =>  ('bs,'k,'r,'v) ins_state option" where
+  "ins_step ctxt1 s0 == (
+case s0 of
+    Down isd => (
+      let r0 = isd|>isd_r in
+      let frm = (page_ref_to_frame (ctxt_p2f_t.truncate ctxt1) (isd|>isd_str) r0) in
+      case frm of
+      None => None
+      | Some frm0 => (
+        case frm0 of
+        Frm_I nf => (  
+          let k2r = ((ctxt1|>key_to_ref)|>dest_key_to_ref) in
+          let r' = k2r nf k0 in (* we need the index *)
+          
+        )
+        | Frm_L lf => None
+      )
+    )
+    | _ => arb
+    
+  )"
+
+
+
+end
+
+
